bedrock2/src/bedrock2/e1000_packet_trace.v
@@ -6,20 +6,36 @@ Require Import coqutil.Word.Interface.
 Require Import coqutil.Datatypes.ZList.
 Require Import bedrock2.ReversedListNotations. Local Open Scope list_scope.
 Import ZList.List.ZIndexNotations. Local Open Scope zlist_scope.
+Require Import bedrock2.SepLib.
 Require Import bedrock2.TraceInspection.
 Require Import bedrock2.RecordPredicates.
 Require Import bedrock2.e1000_state.
 Require Import bedrock2.e1000_read_write_step.
 
-Inductive packet_event: Set :=
-| RxPacket(b: buf)
-| TxPacket(b: buf).
-
 Section WithMem.
   Context {width: Z} {BW: Bitwidth width}
           {word: word.word width} {mem: map.map word Byte.byte}.
 
+  Inductive packet_event: Type :=
+  (* a packet satisfying separation logic predicate p was received: *)
+  | RxPacket(p: word -> mem -> Prop)
+  (* a packet satisfying separation logic predicate p was sent: *)
+  | TxPacket(p: word -> mem -> Prop).
+
   Axiom BootSeq: Semantics.trace.
+
+  (* An element in the receive queue consists of a descriptor with meta data (including
+     the length) and a pointer to a buffer of predefined size containing the actual data,
+     followed by irrelevent data.
+     This function returns the separation logic predicate that only describes the
+     actual (relevant) data in the buffer *)
+  Definition data_of_rxq_elem: rx_desc_t * buf -> word -> mem -> Prop :=
+    fun '(desc, buffer) =>
+      array (uint 8) desc.(rx_desc_length) buffer[:desc.(rx_desc_length)].
+
+  Definition data_of_txq_elem: tx_desc_t * buf -> word -> mem -> Prop :=
+    fun '(desc, buffer) =>
+      array (uint 8) desc.(tx_desc_length) buffer[:desc.(tx_desc_length)].
 
   (* Abstracts a trace of MMIO/DMA events (Semantics.trace)
      into a list of sent/received packets (list packet_event).
@@ -35,7 +51,7 @@ Section WithMem.
       e1000_initialized s t ->
       circular_buffer_slice (rxq_elem s.(rx_buf_size))
             s.(rx_queue_cap) s.(rx_queue_head) rcvd s.(rx_queue_base_addr) mRcv ->
-      packet_trace_rel (pks ;++ List.map (fun '(desc, buffer) => RxPacket buffer) rcvd)
+      packet_trace_rel (pks ;++ List.map (fun e => RxPacket (data_of_rxq_elem e)) rcvd)
         (t ;+ ((map.empty, "memory_mapped_extcall_read32", [|register_address E1000_RDH|]),
                (mRcv, [|newRDH|])))
   (* software provides new receive buffers to NIC: ignored in packet trace *)
@@ -52,7 +68,7 @@ Section WithMem.
       getTDT t oldTDT ->
       circular_buffer_slice txq_elem s.(tx_queue_cap) oldTDT sent
         s.(tx_queue_base_addr) mGive ->
-      packet_trace_rel (pks ;++ List.map (fun '(desc, buffer) => TxPacket buffer) sent)
+      packet_trace_rel (pks ;++ List.map (fun e => TxPacket (data_of_txq_elem e)) sent)
         (t ;+ ((mGive, "memory_mapped_extcall_write32",
                  [|register_address E1000_TDT; newTDT|]),
                (map.empty, nil)))
